\documentclass{article}
\author{Bruno Berastain}
\usepackage{amsmath, amssymb, amsthm}

\begin{document}
\title{Playing With Latex}
\maketitle

\section{Deriving the Quadratic Forumla}
% the spacing between one line and the next is too close
% either fix that or do a left/right align
	Start with the general formula for a quadratic equation\\
	
	\(ax^2 +bx+c = 0\)\\

	Divide by \(a\)\\

	\(x^2 + \frac{b}{a}x + \frac{c}{a} = 0\)\\

	Subtract \(\frac{c}{a}\) from both sides\\

	\(x^2 + \frac{b}{a}x = -\frac{c}{a}\)\\

	Complete the square\\

	\(x^2 + \frac{b}{a}x + \frac{b^2}{4a^2} = \frac{b^2}{4a^2} - \frac{c}{a}\)\\

	Factor on the left, find a common denominator on the right\\

	\((x + \frac{b}{2a})^2 = \frac{b^2}{4a^2} - \frac{4ac}{4a^2}\)\\

	Take the square root of both sides\\

	\(x + \frac{b}{2a} = \pm\sqrt{\frac{b^2 - 4ac}{4a^2}}\)\\

	Subtract \(\frac{b}{2a}\) from both sides\\

	\(x = -\frac{b}{2a} \pm\frac{\sqrt{b^2 - 4ac}}{\sqrt{4a^2}}\)\\

	And reorganize\\

	\(x = \frac{-b \pm \sqrt{b^2 - 4ac}}{2a}\)\\

\section{Deriving Trigonometric Identities}
	Start with the identity\\
\begin{equation}
	\sin^2(\theta) + \cos^2(\theta) = 1
\end{equation}	
	Divide both sides by \(\cos^2(\theta)\)\\

	\(\frac{\sin^2(\theta)}{\cos^2(\theta)} + \frac{\cos^2(\theta)}{\cos^2(\theta)} = \frac{1}{\cos^2(\theta)}\)\\
\begin{equation}
	\tan^2(\theta) + 1 = \sec^2(\theta)
\end{equation}
	Alternatively, start with the same identity and divide both sides by \(\sin^2(\theta)\)\\
	
	\(\frac{\sin^2(\theta)}{\sin^2(\theta)} + \frac{\cos^2(\theta)}{\sin^2(\theta)} = \frac{1}{\sin^2(\theta)}\)\\
\begin{equation}
	1 + \cot^2(\theta) = \csc^2(\theta)
\end{equation}

	Pythagorean Theorem
	\(a^2 + b^2 = c^2\)
	
\end{document}